src/PlutusIR/Extract.v
@@ -1,0 +1,11 @@
+From PlutusCert Require Import
+  DeadCode.DecideBool
+  UniqueBinders.DecOpt.
+
+From Coq Require Import Strings.Ascii.
+From Coq Require Import Extraction.
+Extraction Language Haskell.
+Recursive Extraction
+  dec_Term
+  dec_unique
+  ascii_of_nat.
